Semantic/Capybara/Syntax/Exp.lean
@@ -9,10 +9,9 @@ namespace Capybara
 /-- An expression in CC. -/
 inductive Exp : Sig -> Type where
 | var : Var .var s -> Exp s
-| abs : CaptureSet s -> Ty .capt s -> Exp (s,x) -> Exp s
+| abs : CaptureSet s -> Ty .capt (s,C) -> Exp (s,x) -> Exp s
 | tabs : CaptureSet s -> PureTy s -> Exp (s,X) -> Exp s
 | cabs : CaptureSet s -> CaptureBound s -> Exp (s,C) -> Exp s
-| boxed : CaptureSet s -> SepCtx s -> Exp s -> Exp s
 | reader : Var .var s -> Exp s
 | alloc : Var .var s -> Exp s
 | drop : Var .var s -> Exp s
@@ -20,7 +19,6 @@ inductive Exp : Sig -> Type where
 | app : Var .var s -> Var .var s -> Exp s
 | tapp : Var .var s -> PureTy s -> Exp s
 | capp : Var .var s -> CaptureSet s -> Exp s
-| unwrap : Var .var s -> Exp s
 | letin : Exp s -> Exp (s,x) -> Exp s
 | unpack : Exp s -> Exp ((s,C),x) -> Exp s
 | unit : Exp s
@@ -37,10 +35,9 @@ inductive Exp : Sig -> Type where
 /-- Applies a renaming to all bound variables in an expression. -/
 def Exp.rename : Exp s1 -> Rename s1 s2 -> Exp s2
 | .var x, f => .var (x.rename f)
-| .abs cs T e, f => .abs (cs.rename f) (T.rename f) (e.rename (f.lift))
+| .abs cs T e, f => .abs (cs.rename f) (T.rename (f.lift)) (e.rename (f.lift))
 | .tabs cs T e, f => .tabs (cs.rename f) (T.rename f) (e.rename (f.lift))
 | .cabs cs cb e, f => .cabs (cs.rename f) (cb.rename f) (e.rename (f.lift))
-| .boxed cs Ψ e, f => .boxed (cs.rename f) (Ψ.rename f) (e.rename f)
 | .reader x, f => .reader (x.rename f)
 | .alloc x, f => .alloc (x.rename f)
 | .drop x, f => .drop (x.rename f)
@@ -48,7 +45,6 @@ def Exp.rename : Exp s1 -> Rename s1 s2 -> Exp s2
 | .app x y, f => .app (x.rename f) (y.rename f)
 | .tapp x T, f => .tapp (x.rename f) (T.rename f)
 | .capp x cs, f => .capp (x.rename f) (cs.rename f)
-| .unwrap x, f => .unwrap (x.rename f)
 | .letin e1 e2, f => .letin (e1.rename f) (e2.rename (f.lift))
 | .unpack e1 e2, f => .unpack (e1.rename f) (e2.rename (f.lift.lift))
 | .unit, _ => .unit
@@ -64,7 +60,6 @@ inductive Exp.IsVal : Exp s -> Prop where
 | abs : Exp.IsVal (.abs cs T e)
 | tabs : Exp.IsVal (.tabs cs T e)
 | cabs : Exp.IsVal (.cabs cs m e)
-| boxed : Exp.IsVal (.boxed cs Ψ e)
 | pack : Exp.IsVal (.pack cs x)
 | reader : Exp.IsVal (.reader x)
 | unit : Exp.IsVal .unit
@@ -77,7 +72,6 @@ inductive Exp.IsSimpleVal : Exp s -> Prop where
 | abs : Exp.IsSimpleVal (.abs cs T e)
 | tabs : Exp.IsSimpleVal (.tabs cs T e)
 | cabs : Exp.IsSimpleVal (.cabs cs m e)
-| boxed : Exp.IsSimpleVal (.boxed cs Ψ e)
 | unit : Exp.IsSimpleVal .unit
 | btrue : Exp.IsSimpleVal .btrue
 | bfalse : Exp.IsSimpleVal .bfalse
@@ -108,17 +102,15 @@ def Exp.rename_id {e : Exp s} : e.rename (Rename.id) = e := by
   | var x =>
     simp only [Exp.rename, Var.rename_id]
   | abs cs T e ih =>
-    simp only [Exp.rename, CaptureSet.rename_id, Ty.rename_id, Rename.lift_id]
-    exact congrArg (Exp.abs cs T) ih
+    simp only [Exp.rename, CaptureSet.rename_id, Rename.lift_id]
+    have hT : T.rename Rename.id = T := Ty.rename_id
+    congr 1
   | tabs cs T e ih =>
     simp only [Exp.rename, CaptureSet.rename_id, PureTy.rename_id, Rename.lift_id]
     exact congrArg (Exp.tabs cs T) ih
   | cabs cs cb e ih =>
     simp only [Exp.rename, CaptureSet.rename_id, CaptureBound.rename_id, Rename.lift_id]
     exact congrArg (Exp.cabs cs cb) ih
-  | boxed cs Ψ e ih =>
-    simp only [Exp.rename, CaptureSet.rename_id, SepCtx.rename_id]
-    exact congrArg (Exp.boxed cs Ψ) ih
   | reader x =>
     simp only [Exp.rename, Var.rename_id]
   | alloc x =>
@@ -133,8 +125,6 @@ def Exp.rename_id {e : Exp s} : e.rename (Rename.id) = e := by
     simp only [Exp.rename, Var.rename_id, PureTy.rename_id]
   | capp x cs =>
     simp only [Exp.rename, Var.rename_id, CaptureSet.rename_id]
-  | unwrap x =>
-    simp only [Exp.rename, Var.rename_id]
   | letin e1 e2 ih1 ih2 =>
     simp only [Exp.rename, Rename.lift_id, ih1]
     exact congrArg (Exp.letin e1) ih2
@@ -167,7 +157,7 @@ theorem Exp.rename_comp {e : Exp s1} {f : Rename s1 s2} {g : Rename s2 s3} :
     simp only [Exp.rename, Var.rename_comp]
   | abs cs T e ih =>
     simpa only [Exp.rename, CaptureSet.rename_comp, Ty.rename_comp, Rename.lift_comp] using
-      congrArg (Exp.abs (cs.rename (f.comp g)) (T.rename (f.comp g)))
+      congrArg (Exp.abs (cs.rename (f.comp g)) (T.rename (f.lift.comp g.lift)))
         (ih (f := f.lift) (g := g.lift))
   | tabs cs T e ih =>
     simpa only [Exp.rename, CaptureSet.rename_comp, PureTy.rename_comp, Rename.lift_comp] using
@@ -182,9 +172,6 @@ theorem Exp.rename_comp {e : Exp s1} {f : Rename s1 s2} {g : Rename s2 s3} :
     ] using
       congrArg (Exp.cabs (cs.rename (f.comp g)) (cb.rename (f.comp g)))
         (ih (f := f.lift) (g := g.lift))
-  | boxed cs Ψ e ih =>
-    simpa only [Exp.rename, CaptureSet.rename_comp, SepCtx.rename_comp] using
-      congrArg (Exp.boxed (cs.rename (f.comp g)) (Ψ.rename (f.comp g))) (ih (f := f) (g := g))
   | reader x =>
     simp only [Exp.rename, Var.rename_comp]
   | alloc x =>
@@ -199,8 +186,6 @@ theorem Exp.rename_comp {e : Exp s1} {f : Rename s1 s2} {g : Rename s2 s3} :
     simp only [Exp.rename, Var.rename_comp, PureTy.rename_comp]
   | capp x cs =>
     simp only [Exp.rename, Var.rename_comp, CaptureSet.rename_comp]
-  | unwrap x =>
-    simp only [Exp.rename, Var.rename_comp]
   | letin e1 e2 ih1 ih2 =>
     simpa only [Exp.rename, Rename.lift_comp, ih1] using
       congrArg (Exp.letin (e1.rename (f.comp g))) (ih2 (f := f.lift) (g := g.lift))
@@ -243,8 +228,6 @@ inductive Exp.IsClosed : Exp s -> Prop where
     Exp.IsClosed (.tabs cs T e)
 | cabs : CaptureSet.IsClosed cs -> CaptureBound.IsClosed cb -> Exp.IsClosed e ->
     Exp.IsClosed (.cabs cs cb e)
-| boxed : CaptureSet.IsClosed cs -> SepCtx.IsClosed Ψ -> Exp.IsClosed e ->
-    Exp.IsClosed (.boxed cs Ψ e)
 | reader : Var.IsClosed x -> Exp.IsClosed (.reader x)
 | alloc : Var.IsClosed x -> Exp.IsClosed (.alloc x)
 | drop : Var.IsClosed x -> Exp.IsClosed (.drop x)
@@ -252,7 +235,6 @@ inductive Exp.IsClosed : Exp s -> Prop where
 | app : Var.IsClosed x -> Var.IsClosed y -> Exp.IsClosed (.app x y)
 | tapp : Var.IsClosed x -> PureTy.IsClosed T -> Exp.IsClosed (.tapp x T)
 | capp : Var.IsClosed x -> CaptureSet.IsClosed cs -> Exp.IsClosed (.capp x cs)
-| unwrap : Var.IsClosed x -> Exp.IsClosed (.unwrap x)
 | letin : Exp.IsClosed e1 -> Exp.IsClosed e2 -> Exp.IsClosed (.letin e1 e2)
 | unpack : Exp.IsClosed e1 -> Exp.IsClosed e2 -> Exp.IsClosed (.unpack e1 e2)
 | unit : Exp.IsClosed .unit
